
@prefix dcterms: <http://purl.org/dc/terms/> .
@prefix pescAcademicSummaryTypes: <https://pesc.org/vocabs/AcademicSummaryTypes#> .
@prefix skos: <http://www.w3.org/2004/02/skos/core#> .

pescAcademicSummaryTypes:AcademicRenewal a skos:Concept ;
    skos:definition "Subset of forgiven courses" ;
    skos:inScheme pescAcademicSummaryTypes: ;
    skos:notation "AcademicRenewal" ;
    skos:prefLabel "Academic Renewal" ;
    skos:topConceptOf pescAcademicSummaryTypes: .

pescAcademicSummaryTypes:All a skos:Concept ;
    skos:definition "Summary of all courses regardless of institution" ;
    skos:inScheme pescAcademicSummaryTypes: ;
    skos:notation "All" ;
    skos:prefLabel "All" ;
    skos:topConceptOf pescAcademicSummaryTypes: .

pescAcademicSummaryTypes:AllNotRepeated a skos:Concept ;
    skos:definition "Summary of all courses except for repeated or forgiven courses/credits" ;
    skos:inScheme pescAcademicSummaryTypes: ;
    skos:notation "AllNotRepeated" ;
    skos:prefLabel "All Not Repeated" ;
    skos:topConceptOf pescAcademicSummaryTypes: .

pescAcademicSummaryTypes:CarryoverCredit a skos:Concept ;
    skos:definition "Summary from offline records and used as the intitial point for cumulatives and averages" ;
    skos:inScheme pescAcademicSummaryTypes: ;
    skos:notation "CarryoverCredit" ;
    skos:prefLabel "Carryover Credit" ;
    skos:topConceptOf pescAcademicSummaryTypes: .

pescAcademicSummaryTypes:ConvertedFrom a skos:Concept ;
    skos:definition "Summary of credits before an institutional term-basis conversion, such as from quarters to semesters" ;
    skos:inScheme pescAcademicSummaryTypes: ;
    skos:notation "ConvertedFrom" ;
    skos:prefLabel "Converted From" ;
    skos:topConceptOf pescAcademicSummaryTypes: .

pescAcademicSummaryTypes:ConvertedTo a skos:Concept ;
    skos:definition "Summary of credits after an institutional term-basis conversion, such as from quarters to semesters" ;
    skos:inScheme pescAcademicSummaryTypes: ;
    skos:notation "ConvertedTo" ;
    skos:prefLabel "Converted To" ;
    skos:topConceptOf pescAcademicSummaryTypes: .

pescAcademicSummaryTypes:Cumulative a skos:Concept ;
    skos:definition "Cumulative" ;
    skos:inScheme pescAcademicSummaryTypes: ;
    skos:notation "Cumulative" ;
    skos:prefLabel "Cumulative" ;
    skos:topConceptOf pescAcademicSummaryTypes: .

pescAcademicSummaryTypes:DegreeApplicable a skos:Concept ;
    skos:definition "Summary of course that apply to degree" ;
    skos:inScheme pescAcademicSummaryTypes: ;
    skos:notation "DegreeApplicable" ;
    skos:prefLabel "Degree Applicable" ;
    skos:topConceptOf pescAcademicSummaryTypes: .

pescAcademicSummaryTypes:NonDegreeApplicable a skos:Concept ;
    skos:definition "Summary of courses that do not apply toward degree" ;
    skos:inScheme pescAcademicSummaryTypes: ;
    skos:notation "NonDegreeApplicable" ;
    skos:prefLabel "Non Degree Applicable" ;
    skos:topConceptOf pescAcademicSummaryTypes: .

pescAcademicSummaryTypes:NonWeighted a skos:Concept ;
    skos:definition "Summary that does not give additional value to courses, regardless of special characteristics of the courses. For example, if the grading scale is from 0 to 4.00, then it is not possible to have a summary higher than 4.00." ;
    skos:inScheme pescAcademicSummaryTypes: ;
    skos:notation "NonWeighted" ;
    skos:prefLabel "Non Weighted" ;
    skos:topConceptOf pescAcademicSummaryTypes: .

pescAcademicSummaryTypes:SenderNotRepeated a skos:Concept ;
    skos:definition "Summary of all courses at sending institution except for repeated or forgiven courses/credits" ;
    skos:inScheme pescAcademicSummaryTypes: ;
    skos:notation "SenderNotRepeated" ;
    skos:prefLabel "Sender Not Repeated" ;
    skos:topConceptOf pescAcademicSummaryTypes: .

pescAcademicSummaryTypes:SenderOnly a skos:Concept ;
    skos:definition "Summary of all courses at sending institution (or recorded as if they were taken at the" ;
    skos:inScheme pescAcademicSummaryTypes: ;
    skos:notation "SenderOnly" ;
    skos:prefLabel "Sender Only" ;
    skos:topConceptOf pescAcademicSummaryTypes: .

pescAcademicSummaryTypes:TransferNotRepeated a skos:Concept ;
    skos:definition "Summary of transfer work except for repeated or forgiven courses/credits" ;
    skos:inScheme pescAcademicSummaryTypes: ;
    skos:notation "TransferNotRepeated" ;
    skos:prefLabel "Transfer Not Repeated" ;
    skos:topConceptOf pescAcademicSummaryTypes: .

pescAcademicSummaryTypes:TransferOnly a skos:Concept ;
    skos:definition "Summary of transfer work (courses taken at other than the sending institution)" ;
    skos:inScheme pescAcademicSummaryTypes: ;
    skos:notation "TransferOnly" ;
    skos:prefLabel "Transfer Only" ;
    skos:topConceptOf pescAcademicSummaryTypes: .

pescAcademicSummaryTypes:UserDefined a skos:Concept ;
    skos:definition "see NoteMessage for explanation." ;
    skos:inScheme pescAcademicSummaryTypes: ;
    skos:notation "UserDefined" ;
    skos:prefLabel "User Defined" ;
    skos:topConceptOf pescAcademicSummaryTypes: .

pescAcademicSummaryTypes:Weighted a skos:Concept ;
    skos:definition "Summary that gives additional (higher) value to specific courses taken by a student, such as honors courses, International Baccalaureate, Advanced Placement, high school /college dual enrollment." ;
    skos:inScheme pescAcademicSummaryTypes: ;
    skos:notation "Weighted" ;
    skos:prefLabel "Weighted" ;
    skos:topConceptOf pescAcademicSummaryTypes: .

pescAcademicSummaryTypes: a skos:ConceptScheme ;
    dcterms:description "Summary Type is an indication of what is being summarized over which period of time." ;
    dcterms:title "Academic Summary Types" ;
    skos:hasTopConcept pescAcademicSummaryTypes:AcademicRenewal,
        pescAcademicSummaryTypes:All,
        pescAcademicSummaryTypes:AllNotRepeated,
        pescAcademicSummaryTypes:CarryoverCredit,
        pescAcademicSummaryTypes:ConvertedFrom,
        pescAcademicSummaryTypes:ConvertedTo,
        pescAcademicSummaryTypes:Cumulative,
        pescAcademicSummaryTypes:DegreeApplicable,
        pescAcademicSummaryTypes:NonDegreeApplicable,
        pescAcademicSummaryTypes:NonWeighted,
        pescAcademicSummaryTypes:SenderNotRepeated,
        pescAcademicSummaryTypes:SenderOnly,
        pescAcademicSummaryTypes:TransferNotRepeated,
        pescAcademicSummaryTypes:TransferOnly,
        pescAcademicSummaryTypes:UserDefined,
        pescAcademicSummaryTypes:Weighted .

