
@prefix dcterms: <http://purl.org/dc/terms/> .
@prefix pescAccreditationBodyCodes: <https://pesc.org/vocabs/AccreditationBodyCodes#> .
@prefix skos: <http://www.w3.org/2004/02/skos/core#> .

pescAccreditationBodyCodes:MSA a skos:Concept ;
    skos:definition "Middle States Association of Colleges and Schools, Commission on Higher Education" ;
    skos:inScheme pescAccreditationBodyCodes: ;
    skos:notation "MSA" ;
    skos:prefLabel "Msa" ;
    skos:topConceptOf pescAccreditationBodyCodes: .

pescAccreditationBodyCodes:NCA-CASI a skos:Concept ;
    skos:definition "North Central Association of Colleges and Schools, Commission on Accreditation and School Improvement, Board of Trustees" ;
    skos:inScheme pescAccreditationBodyCodes: ;
    skos:notation "NCA-CASI" ;
    skos:prefLabel "Nca-Casi" ;
    skos:topConceptOf pescAccreditationBodyCodes: .

pescAccreditationBodyCodes:NCA-HLC a skos:Concept ;
    skos:definition "North Central Association of Colleges and Schools, Higher Learning Commission" ;
    skos:inScheme pescAccreditationBodyCodes: ;
    skos:notation "NCA-HLC" ;
    skos:prefLabel "Nca-Hlc" ;
    skos:topConceptOf pescAccreditationBodyCodes: .

pescAccreditationBodyCodes:NEASC-CIHE a skos:Concept ;
    skos:definition "New England Association of Schools and Colleges, Inc., Commission on Institutions of Higher Education" ;
    skos:inScheme pescAccreditationBodyCodes: ;
    skos:notation "NEASC-CIHE" ;
    skos:prefLabel "Neasc-Cihe" ;
    skos:topConceptOf pescAccreditationBodyCodes: .

pescAccreditationBodyCodes:NEASC-CTCI a skos:Concept ;
    skos:definition "New England Association of Schools and Colleges, Inc., Commission on Technical and Career Institutions" ;
    skos:inScheme pescAccreditationBodyCodes: ;
    skos:notation "NEASC-CTCI" ;
    skos:prefLabel "Neasc-Ctci" ;
    skos:topConceptOf pescAccreditationBodyCodes: .

pescAccreditationBodyCodes:NWCCU a skos:Concept ;
    skos:definition "Northwest Commission on Colleges and Universities" ;
    skos:inScheme pescAccreditationBodyCodes: ;
    skos:notation "NWCCU" ;
    skos:prefLabel "Nwccu" ;
    skos:topConceptOf pescAccreditationBodyCodes: .

pescAccreditationBodyCodes:Other a skos:Concept ;
    skos:definition "Use AccreditationTypeName to enter Accrediting body other than listed" ;
    skos:inScheme pescAccreditationBodyCodes: ;
    skos:notation "Other" ;
    skos:prefLabel "Other" ;
    skos:topConceptOf pescAccreditationBodyCodes: .

pescAccreditationBodyCodes:SACS a skos:Concept ;
    skos:definition "Southern Association of Colleges and Schools, Commission on Colleges" ;
    skos:inScheme pescAccreditationBodyCodes: ;
    skos:notation "SACS" ;
    skos:prefLabel "Sacs" ;
    skos:topConceptOf pescAccreditationBodyCodes: .

pescAccreditationBodyCodes:WASC-ACCJC a skos:Concept ;
    skos:definition "Western Association of Schools and Colleges, Accrediting Commission for Community and Junior Colleges" ;
    skos:inScheme pescAccreditationBodyCodes: ;
    skos:notation "WASC-ACCJC" ;
    skos:prefLabel "Wasc-Accjc" ;
    skos:topConceptOf pescAccreditationBodyCodes: .

pescAccreditationBodyCodes:WASC-ACSCU a skos:Concept ;
    skos:definition "Western Association of Schools and Colleges, Accrediting Commission for Senior Colleges and Universities" ;
    skos:inScheme pescAccreditationBodyCodes: ;
    skos:notation "WASC-ACSCU" ;
    skos:prefLabel "Wasc-Acscu" ;
    skos:topConceptOf pescAccreditationBodyCodes: .

pescAccreditationBodyCodes: a skos:ConceptScheme ;
    dcterms:description "Need Definition" ;
    dcterms:title "Accreditation Body Codes" ;
    skos:hasTopConcept pescAccreditationBodyCodes:MSA,
        pescAccreditationBodyCodes:NCA-CASI,
        pescAccreditationBodyCodes:NCA-HLC,
        pescAccreditationBodyCodes:NEASC-CIHE,
        pescAccreditationBodyCodes:NEASC-CTCI,
        pescAccreditationBodyCodes:NWCCU,
        pescAccreditationBodyCodes:Other,
        pescAccreditationBodyCodes:SACS,
        pescAccreditationBodyCodes:WASC-ACCJC,
        pescAccreditationBodyCodes:WASC-ACSCU .

